execution/examples/BoardroomVoting.v
@@ -808,7 +808,10 @@ Proof.
       rewrite queue_prev in H2.
       cbn in H2.
       destruct (address_eqb_spec (act_from act) to_addr); cbn in *; try congruence.
-      subst act; cbn in *; congruence.
+      match goal with
+      | [ H : act = _ |- _ ] => rewrite H in *
+      end.
+      cbn in *; congruence.
 Qed.
 
 Theorem boardroom_voting_correct
