execution/tests/ChainPrinters.v
@@ -156,6 +156,7 @@ Instance showAddBlockError `{Show (@Action Base)} : Show AddBlockError :=
   show err := match err with
               | invalid_header => "invalid_header"
               | invalid_root_action act => "invalid_root_action: " ++ show act
+              | origin_from_mismatch act => "origin_from_mismatch: " ++ show act
               | action_evaluation_depth_exceeded => "action_evaluation_depth_exceeded"
               | action_evaluation_error act eval_error =>
                 "action_evaluation_error for " ++ show act ++ " with error: " ++ show eval_error
