execution/tests/FA2Tests/FA2TokenTests.v
@@ -91,41 +91,41 @@ Definition client_contract_addr : Address := BoundedN.of_Z_const AddrSize 129%Z.
 Definition chain_with_token_deployed_with_hook : ChainBuilder :=
   unpack_result (TraceGens.add_block (lcb_initial AddrSize)
   [
-    build_act creator (act_transfer person_1 10);
-    build_act creator (act_transfer person_2 10);
-    build_act creator (act_transfer person_3 10);
-    build_act creator deploy_fa2token_with_transfer_hook;
-    build_act creator deploy_fa2token_client;
-    build_act creator deploy_fa2hook
+    build_act creator eq_refl creator (act_transfer person_1 10);
+    build_act creator eq_refl creator (act_transfer person_2 10);
+    build_act creator eq_refl creator (act_transfer person_3 10);
+    build_act creator eq_refl creator deploy_fa2token_with_transfer_hook;
+    build_act creator eq_refl creator deploy_fa2token_client;
+    build_act creator eq_refl creator deploy_fa2hook
   ]).
 
 Definition chain_with_token_deployed_without_hook : ChainBuilder :=
   unpack_result (TraceGens.add_block (lcb_initial AddrSize)
   [
-    build_act creator (act_transfer person_1 10);
-    build_act creator (act_transfer person_2 10);
-    build_act creator (act_transfer person_3 10);
-    build_act creator deploy_fa2token_without_transfer_hook;
-    build_act creator deploy_fa2token_client
+    build_act creator eq_refl creator (act_transfer person_1 10);
+    build_act creator eq_refl creator (act_transfer person_2 10);
+    build_act creator eq_refl creator (act_transfer person_3 10);
+    build_act creator eq_refl creator deploy_fa2token_without_transfer_hook;
+    build_act creator eq_refl creator deploy_fa2token_client
   ]).
 
 Definition chain_without_transfer_hook' : result ChainBuilder AddBlockError :=
   (TraceGens.add_block chain_with_token_deployed_without_hook
   [
-    build_act person_1 (act_call token_contract_base_addr 10%Z (serialize _ _ (msg_create_tokens 0%N))) ;
-    build_act person_2 (act_call token_contract_base_addr 10%Z (serialize _ _ (msg_create_tokens 0%N)))
+    build_act person_1 eq_refl person_1 (act_call token_contract_base_addr 10%Z (serialize _ _ (msg_create_tokens 0%N))) ;
+    build_act person_2 eq_refl person_2 (act_call token_contract_base_addr 10%Z (serialize _ _ (msg_create_tokens 0%N)))
   ]).
 
 Definition chain_with_transfer_hook' : result ChainBuilder AddBlockError :=
   (TraceGens.add_block chain_with_token_deployed_with_hook
   [
-    build_act person_1 (act_call token_contract_base_addr 10%Z (serialize _ _ (msg_create_tokens 0%N))) ;
-    build_act person_2 (act_call token_contract_base_addr 10%Z (serialize _ _ (msg_create_tokens 0%N)))
+    build_act person_1 eq_refl person_1 (act_call token_contract_base_addr 10%Z (serialize _ _ (msg_create_tokens 0%N))) ;
+    build_act person_2 eq_refl person_2 (act_call token_contract_base_addr 10%Z (serialize _ _ (msg_create_tokens 0%N)))
   ]).
 
-(* Uncomment for testing. This is commented because it is computationally expensive (> 20 seconds to compute) *)
-(* Definition chain_without_transfer_hook := unpack_result chain_without_transfer_hook'. *)
-(* Definition chain_without_transfer_hook := unpack_result chain_without_transfer_hook'. *)
+Definition chain_without_transfer_hook := unpack_result chain_without_transfer_hook'.
+Definition chain_with_transfer_hook := unpack_result chain_with_transfer_hook'.
+
 
 Definition client_other_msg := @other_msg _ FA2ClientMsg _.
 
@@ -232,11 +232,11 @@ Definition post_transfer_correct (chain : Chain) (cctx : ContractCallContext) ol
   | None => checker false
   end.
 
-(* QuickChick (
-  {{ msg_is_transfer }}
-    token_contract_base_addr
-  {{ post_transfer_correct }}
-  chain_without_transfer_hook). *)
+(* QuickChick ( *)
+(*   {{ msg_is_transfer }} *)
+(*     token_contract_base_addr *)
+(*   {{ post_transfer_correct }} *)
+(*   chain_without_transfer_hook). *)
 (* 14 seconds, max size 7, 1 act per block *)
 (* +++ Passed 10000 tests (0 discards) *)
 
